# baseURI: http://linked.data.gov.au/def/placenames
# imports: http://www.opengis.net/ont/geosparql

@prefix : <http://linked.data.gov.au/def/placenames/> .
@prefix dcterms: <http://purl.org/dc/terms/> .
@prefix ex: <http://linked.data.gov.au/dataset/placename/> .
@prefix geo: <http://www.opengis.net/ont/geosparql#> .
@prefix loci: <http://linked.data.gov.au/def/loci#> .
@prefix owl: <http://www.w3.org/2002/07/owl#> .
@prefix prof: <http://www.w3.org/ns/dx/prof/> .
@prefix prov: <http://www.w3.org/ns/prov#> .
@prefix pt: <http://linked.data.gov.au/def/placetype/> .
@prefix rdf: <http://www.w3.org/1999/02/22-rdf-syntax-ns#> .
@prefix rdfs: <http://www.w3.org/2000/01/rdf-schema#> .
@prefix reg: <http://purl.org/linked-data/registry#> .
@prefix schema: <https://schema.org/> .
@prefix sf: <http://www.opengis.net/ont/sf#> .
@prefix skos: <http://www.w3.org/2004/02/skos/core#> .
@prefix vann: <http://purl.org/vocab/vann/> .
@prefix xml: <http://www.w3.org/XML/1998/namespace> .
@prefix xsd: <http://www.w3.org/2001/XMLSchema#> .

ex:Ayers-Rock
  a :OfficialPlaceName ;
  loci:isMemberOf <https://www.ntlis.nt.gov.au/placenames/> ;
  :dateGazetted "1850-01-01"^^xsd:date ;
  :dateRetired "1989-12-31"^^xsd:date ;
  :name "Ayers Rock"@en ;
  :placeNameOf ex:NT_10532 ;
  :status :retired ;
  :wasNamedBy <https://www.ntlis.nt.gov.au/placenames/> ;
  rdfs:comment "NOTE: EXAMPLE ONLY DETAILS MAY BE INCORRECT" ;
  rdfs:label "Ayers Rock" ;
.
ex:Ayers-Rock-Uluru
  a :OfficialPlaceName ;
  loci:isMemberOf <https://www.ntlis.nt.gov.au/placenames/> ;
  :dateGazetted "1990-01-01"^^xsd:date ;
  :dateRetired "2005-12-31"^^xsd:date ;
  :name "Ayers Rock / Uluru"@en ;
  :placeNameOf ex:NT_10532 ;
  :status :retired ;
  :wasNamedBy <https://www.ntlis.nt.gov.au/placenames/> ;
  rdfs:comment "NOTE: EXAMPLE ONLY DETAILS MAY BE INCORRECT" ;
  rdfs:label "Ayers Rock (Uluru)" ;
.
ex:DH
  a :PlaceName ;
  :name "The cubby house"@en ;
  :placeNameOf ex:INF9987234 ;
  :status :informal ;
  :wasNamedBy <https://people.example.org/fagin> ;
  rdfs:comment "NOTE: EXAMPLE ONLY " ;
  rdfs:label "The cubby house" ;
.
ex:INF9987234
  a :Place ;
  dcterms:identifier "INF9987234" ;
  dcterms:type <http://pid.geoscience.gov.au/def/voc/ga/PlaceType/UNCLASSIFIED> ;
  geo:hasGeometry [
      a sf:Point ;
      geo:asWKT "POINT (145.029494308 -37.907730551)"^^geo:wktLiteral ;
    ] ;
.
ex:NT_10532
  a :Place ;
  :hasPlaceClassification <http://pid.geoscience.gov.au/def/voc/ga/PlaceType/MOUNTAIN> ;
  :hasPlaceName ex:Ayers-Rock ;
  :hasPlaceName ex:Ayers-Rock-Uluru ;
  :hasPlaceName ex:Uluru-Ayers-Rock ;
  dcterms:identifier "NT_10532" ;
  geo:hasGeometry [
      a <http://linked.data.gov.au/def/auspix#Geometry> ;
      rdfs:member <http://ec2-52-63-73-113.ap-southeast-2.compute.amazonaws.com/AusPIX-DGGS-dataset/ausPIX/R7430551> ;
    ] ;
  geo:hasGeometry [
      a sf:Point ;
      geo:asWKT "POINT(-25.3415 131.0354)"^^geo:wktLiteral ;
    ] ;
  rdfs:seeAlso <http://ec2-52-63-73-113.ap-southeast-2.compute.amazonaws.com/placenames-dataset/placename/NT_10532> ;
.
ex:Uluru-Ayers-Rock
  a :OfficialPlaceName ;
  loci:isMemberOf <https://www.ntlis.nt.gov.au/placenames/> ;
  :dateGazetted "2006-01-01"^^xsd:date ;
  :name "Uluru / Ayers Rock"@pjt ;
  :placeNameOf ex:NT_10532 ;
  :status :gazetted ;
  :wasNamedBy <https://www.ntlis.nt.gov.au/placenames/> ;
  rdfs:comment "NOTE: EXAMPLE ONLY DETAILS MAY BE INCORRECT" ;
  rdfs:label "Uluru (Ayers Rock)" ;
.
loci:Dataset
  a owl:Class ;
.
loci:isMemberOf
  a owl:ObjectProperty ;
.
<http://linked.data.gov.au/def/placenames>
  a owl:NamedIndividual ;
  a owl:Ontology ;
  dcterms:contributor <https://orcid.org/0000-0002-4643-7289> ;
  dcterms:contributor <https://orcid.org/0000-0003-3425-0780> ;
  dcterms:created "2018-08-02"^^xsd:date ;
  dcterms:creator <https://orcid.org/0000-0002-3884-3420> ;
  dcterms:creator <https://orcid.org/0000-0002-8742-7730> ;
  dcterms:modified "2020-08-27"^^xsd:date ;
  dcterms:publisher [
      rdfs:seeAlso <https://www.ga.gov.au> ;
      schema:identifier "http://catalogue.linked.data.gov.au/org/ga" ;
      schema:name "Geoscience Australia" ;
    ] ;
  dcterms:rights "(c) Commonwealth of Australia (Geoscience Australia) 2019, 2020" ;
  dcterms:title "Place Names Ontology"@en ;
  rdfs:comment """**Place Names** is an RDF/OWL Ontology to define the structure and relationship of the names of geospatial features, typically collected in a Gazetteer.

A **place-name** is a text string that is 

- assigned by an agent (person or organization)
- assigned a designated 'status', with default=\"informal\"
- denotes a natural or constructed geospatial feature 

An **official place-name** is a place-name that 

- is authorized by a place-naming-authority, often a jurisidiction (national, state or local government) 
- is a member item in a gazetteer
- has lifecycle information (status, dates) 
- denotes a natural or constructed geospatial feature with a specified classification (inhabited place, administrative area, mountain, school, station, park ...)

This ontology uses classes and properties from existing vocabularies, in particular

- [GeoSPARQL](http://www.opengis.net/ont/geosparql)
- [SKOS](http://www.w3.org/2004/02/skos/core) 
- [Dublin Core](https://www.dublincore.org/specifications/dublin-core/dcmi-terms/)

![](./images/placename-details.png)""" ;
  rdfs:label "Place Names Ontology"@en ;
  owl:imports <http://www.opengis.net/ont/geosparql> ;
  prof:hasResource [
      dcterms:format <https://w3id.org/mediatype/text/html> ;
      prof:hasArtifact <http://linked.data.gov.au/def/placenames> ;
      prof:hasRole <http://www.w3.org/ns/dx/prof/role/specification> ;
    ] ;
  prof:hasResource [
      dcterms:format <https://w3id.org/mediatype/text/turtle> ;
      prof:hasArtifact <http://linked.data.gov.au/def/placenames.ttl> ;
      prof:hasRole <http://www.w3.org/ns/dx/prof/role/schema> ;
    ] ;
  prof:isProfileOf <http://www.opengis.net/doc/IS/geosparql/1.0> ;
.
<http://linked.data.gov.au/def/placenames.ttl>
  a owl:NamedIndividual ;
.
:Gazetteer
  a owl:Class ;
  rdfs:comment "A Gazetteer is a list of Place Names"@en ;
  rdfs:label "Gazetteer"@en ;
  rdfs:subClassOf loci:Dataset ;
  rdfs:subClassOf [
      a owl:Restriction ;
      owl:allValuesFrom :PlaceName ;
      owl:onProperty rdfs:member ;
    ] ;
.
:Jurisdiction
  a owl:Class ;
  rdfs:comment "Local, State, Territory or National (Commonwealth) Government that has authority to formally establish (i.e. gazette) place names within its jurisdictional area."@en ;
  rdfs:label "Jurisdiction" ;
  rdfs:subClassOf :PlaceNamingAuthority ;
.
:OfficialPlaceName
  a owl:Class ;
  rdfs:comment "The name of a place, assigned by an official naming authority and included in the Place Names Gazetteer of Australia."@en ;
  rdfs:label "Official place-name" ;
  rdfs:subClassOf :PlaceName ;
  rdfs:subClassOf [
      a owl:Class ;
      owl:complementOf [
          a owl:Restriction ;
          owl:hasValue :informal ;
          owl:onProperty :status ;
        ] ;
    ] ;
  rdfs:subClassOf [
      a owl:Restriction ;
      rdfs:comment "An official placename must be associated with a place-naming-authority. Additional attributions may also be attached." ;
      owl:onProperty :wasNamedBy ;
      owl:someValuesFrom :PlaceNamingAuthority ;
    ] ;
  rdfs:subClassOf [
      a owl:Restriction ;
      owl:cardinality "1"^^xsd:nonNegativeInteger ;
      owl:onProperty :dateGazetted ;
    ] ;
  rdfs:subClassOf [
      a owl:Restriction ;
      owl:cardinality "1"^^xsd:nonNegativeInteger ;
      owl:onProperty :status ;
    ] ;
  rdfs:subClassOf [
      a owl:Restriction ;
      owl:maxCardinality "1"^^xsd:nonNegativeInteger ;
      owl:onProperty :datePublished ;
    ] ;
  rdfs:subClassOf [
      a owl:Restriction ;
      owl:maxCardinality "1"^^xsd:nonNegativeInteger ;
      owl:onProperty :dateReleased ;
    ] ;
  rdfs:subClassOf [
      a owl:Restriction ;
      owl:maxCardinality "1"^^xsd:nonNegativeInteger ;
      owl:onProperty :dateRetired ;
    ] ;
  rdfs:subClassOf [
      a owl:Restriction ;
      owl:onProperty loci:isMemberOf ;
      owl:someValuesFrom :Gazetteer ;
    ] ;
  skos:example """
ex:Ayers-Rock
  rdf:type :PlaceName ;
  rdf:type :OfficialPlaceName ;
  loci:isMemberOf <https://www.ntlis.nt.gov.au/placenames/> ;
  :dateGazetted \"1850-01-01\"^^xsd:date ;
  :dateRetired \"1989-12-31\"^^xsd:date ;
  :name \"Ayers Rock\"@en-AU ;
  :placeNameOf ex:NT_10532 ;
  :status :retired ;
  :wasNamedBy <https://www.ntlis.nt.gov.au/placenames/> ;
  rdfs:label \"Ayers Rock\"@en ;
.

ex:Ayers-Rock-Uluru
  rdf:type :PlaceName ;
  rdf:type :OfficialPlaceName ;
  loci:isMemberOf <https://www.ntlis.nt.gov.au/placenames/> ;
  :dateGazetted \"1990-01-01\"^^xsd:date ;
  :dateRetired \"2005-12-31\"^^xsd:date ;
  :name \"Ayers Rock / Uluru\"@en-AU ;
  :placeNameOf ex:NT_10532 ;
  :status :retired ;
  :wasNamedBy <https://www.ntlis.nt.gov.au/placenames/> ;
  rdfs:label \"Ayers Rock / Uluru\" ;
.

ex:Uluru-Ayers-Rock
  rdf:type :PlaceName ;
  rdf:type :OfficialPlaceName ;
  loci:isMemberOf <https://www.ntlis.nt.gov.au/placenames/> ;
  :dateGazetted \"2006-01-01\"^^xsd:date ;
  :isIndigenous true ;
  :name \"Uluru / Ayers Rock\"@pjt ;
  :placeNameOf ex:NT_10532 ;
  :status :gazetted ;
  :wasNamedBy <https://www.ntlis.nt.gov.au/placenames/> ;
  rdfs:label \"Uluru / Ayers Rock\" ;
.
""" ;
.
:Place
  a owl:Class ;
  rdfs:comment "An identifiable geographic Place as defined by the Composite Gazetteer of Australia. A Place is classified according to an extensible set of types."@en ;
  rdfs:label "Place"@en ;
  rdfs:subClassOf geo:Feature ;
  rdfs:subClassOf [
      a owl:Restriction ;
      owl:minCardinality "1"^^xsd:nonNegativeInteger ;
      owl:onProperty :hasPlaceClassification ;
    ] ;
  rdfs:subClassOf [
      a owl:Restriction ;
      owl:minCardinality "1"^^xsd:nonNegativeInteger ;
      owl:onProperty dcterms:identifier ;
    ] ;
  rdfs:subClassOf [
      a owl:Restriction ;
      owl:minCardinality "1"^^xsd:nonNegativeInteger ;
      owl:onProperty geo:hasGeometry ;
    ] ;
  skos:example """
ex:NT_10532
  rdf:type :Place ;
  :hasPlaceClassification <http://pid.geoscience.gov.au/def/voc/ga/PlaceType/MOUNTAIN> ;
  :hasPlaceName ex:Ayers-Rock ;
  :hasPlaceName ex:Ayers-Rock-Uluru ;
  :hasPlaceName ex:Uluru-Ayers-Rock ;
  dcterms:identifier \"NT_10532\" ;
  geo:hasGeometry [
      rdf:type geo:Geometry ;
      geo:asDGGS \"R7430551\"^^geox:dggsLiteral ;
    ] ;
  geo:hasGeometry [
      rdf:type sf:Point ;
      geo:asWKT \"POINT(-25.3415 131.0354)\"^^geo:wktLiteral ;
    ] ;
  rdfs:seeAlso <http://ec2-52-63-73-113.ap-southeast-2.compute.amazonaws.com/placenames-dataset/placename/NT_10532> ;
.
""" ;
.
:PlaceName
  a owl:Class ;
  rdfs:comment """A name associated with a geospatial place or feature. 

Additional properties are specified for  the sub-class OfficialPlaceName which should be used for formal names"""@en ;
  rdfs:label "Place Name"@en ;
  rdfs:subClassOf [
      a owl:Restriction ;
      owl:cardinality "1"^^xsd:nonNegativeInteger ;
      owl:onProperty :name ;
    ] ;
  rdfs:subClassOf [
      a owl:Restriction ;
      owl:minCardinality "1"^^xsd:nonNegativeInteger ;
      owl:onProperty :placeNameOf ;
    ] ;
  rdfs:subClassOf [
      a owl:Restriction ;
      owl:minCardinality "1"^^xsd:nonNegativeInteger ;
      owl:onProperty dcterms:identifier ;
    ] ;
  skos:example """
ex:DH
  rdf:type :PlaceName ;
  :isIndigenous false ;
  :name \"The cubby house\"@en ;
  :placeNameOf ex:INF9987234 ;
  :status :informal ;
  :wasNamedBy <https://people.example.org/fagin> ;
.""" ;
.
:PlaceNamingAuthority
  a owl:Class ;
  rdfs:comment "Agency or organization that has authority to formally establish place names within its scope."@en ;
  rdfs:label "Naming Authority" ;
  rdfs:subClassOf dcterms:Agent ;
.
:PlaceType
  a owl:Class ;
  rdfs:comment "The classification of a place, from the ICSM Permanent Committee on Place Names classification scheme."@en ;
  rdfs:label "Place Type"@en ;
  rdfs:subClassOf skos:Concept ;
.
:Status
  a owl:Class ;
  rdfs:comment """Status of resource, in context of a standard lifecycle: informal, official, gazetted, released, published, retired

![](./images/status.png)""" ;
  rdfs:label "Status" ;
  rdfs:subClassOf skos:Concept ;
.
:dateGazetted
  a owl:DatatypeProperty ;
  rdfs:comment "Date that the item was gazetted" ;
  rdfs:domain :OfficialPlaceName ;
  rdfs:label "date gazetted" ;
  rdfs:range xsd:date ;
  rdfs:subPropertyOf dcterms:date ;
.
:datePublished
  a owl:DatatypeProperty ;
  rdfs:comment "Date that the item was published" ;
  rdfs:domain :OfficialPlaceName ;
  rdfs:label "date published" ;
  rdfs:range xsd:date ;
  rdfs:subPropertyOf dcterms:date ;
.
:dateReleased
  a owl:DatatypeProperty ;
  rdfs:comment "Date that the item was released" ;
  rdfs:domain :OfficialPlaceName ;
  rdfs:label "date released" ;
  rdfs:range xsd:date ;
  rdfs:subPropertyOf dcterms:date ;
.
:dateRetired
  a owl:DatatypeProperty ;
  rdfs:comment "Date that the item was retired" ;
  rdfs:domain :OfficialPlaceName ;
  rdfs:label "date retired" ;
  rdfs:range xsd:date ;
  rdfs:subPropertyOf dcterms:date ;
.
:gazetted
  a :Status ;
  a owl:NamedIndividual ;
  rdfs:label "gazetted" ;
  skos:prefLabel "gazetted" ;
.
:hasPlaceClassification
  a owl:ObjectProperty ;
  rdfs:comment "A relation between a Place and a classification of its real world phenomena."@en ;
  rdfs:domain :Place ;
  rdfs:label "has place classification" ;
  rdfs:range :PlaceType ;
  rdfs:subPropertyOf dcterms:type ;
.
:hasPlaceName
  a owl:ObjectProperty ;
  rdfs:comment "The Feature has a place name (label) assigned to it"@en ;
  rdfs:domain :Place ;
  rdfs:label "has place name"@en ;
  rdfs:range :PlaceName ;
  owl:inverseOf :placeNameOf ;
  skos:scopeNote "All PlaceName objects names indicated by hasPlaceName should have the role of the name indicated with a Name Type"@en ;
.
:hasPronunciation
  a owl:DatatypeProperty ;
  rdfs:comment "The pronunciation of a Place Name, indicated by means of a phonetic alphabet string"@en ;
  rdfs:domain :PlaceName ;
  rdfs:label "pronunciation"@en ;
  rdfs:range xsd:string ;
.
:informal
  a :Status ;
  a owl:NamedIndividual ;
  rdfs:label "informal" ;
  skos:prefLabel "Informal" ;
.
:isIndigenous
  a owl:DatatypeProperty ;
  rdfs:comment "Flag to indicate if the name is indigenous" ;
  rdfs:domain :PlaceName ;
  rdfs:label "name is indigenous" ;
  rdfs:range xsd:boolean ;
.
:name
  a owl:DatatypeProperty ;
  rdfs:comment """It is recommended to include the language tag on the name value. This will be the IETF code @en-AU for most official names. 

For indigenous names, many of the Australian indigenous languages catalogued by AUSTLANG have official ISO 639-3 codes which may be used as the language tag. 
The ISO 639 codes are available from https://iso639-3.sil.org/about 

For example
- wbv Wajarri https://iso639-3.sil.org/code/wbv
- wdj Wadjiginy  https://iso639-3.sil.org/code/wdj 
- wdu Wadjigu  https://iso639-3.sil.org/code/wdu 
- wgg Wangkangurru https://iso639-3.sil.org/code/wgg """ ;
  rdfs:domain :PlaceName ;
  rdfs:label "name" ;
  rdfs:range rdf:langString ;
.
:official
  a :Status ;
  a owl:NamedIndividual ;
  rdfs:label "official" ;
  skos:narrower :gazetted ;
  skos:narrower :published ;
  skos:narrower :released ;
  skos:narrower :retired ;
  skos:prefLabel "official" ;
.
:placeNameOf
  a owl:ObjectProperty ;
  rdfs:domain :PlaceName ;
  rdfs:label "place name of" ;
  rdfs:range :Place ;
.
:published
  a :Status ;
  a owl:NamedIndividual ;
  rdfs:label "published" ;
  skos:prefLabel "published" ;
.
:released
  a :Status ;
  a owl:NamedIndividual ;
  rdfs:label "released" ;
  skos:prefLabel "released" ;
.
:retired
  a :Status ;
  a owl:NamedIndividual ;
  rdfs:label "retired" ;
  skos:altLabel "historical" ;
  skos:prefLabel "retired" ;
.
:status
  a owl:ObjectProperty ;
  rdfs:label "has status" ;
  rdfs:range :Status ;
  skos:scopeNote "This property indicates the status of a Place Name."@en ;
.
:wasNamedBy
  a owl:ObjectProperty ;
  rdfs:comment "The Agent (person, community, organization) that assigned the name to the Place"@en ;
  rdfs:domain :PlaceName ;
  rdfs:label "was named by"@en ;
  rdfs:range dcterms:Agent ;
  rdfs:subPropertyOf prov:wasAttributedTo ;
.
<https://orcid.org/0000-0002-3884-3420>
  a owl:NamedIndividual ;
  a schema:Person ;
  schema:affiliation [
      schema:identifier "http://catalogue.linked.data.gov.au/org/csiro"^^xsd:anyURI ;
      schema:name "CSIRO" ;
    ] ;
  schema:email <mailto:simon.cox@csiro.au> ;
  schema:identifier "https://orcid.org/0000-0002-3884-3420"^^xsd:anyURI ;
  schema:name "Simon J D Cox"@en ;
.
<https://orcid.org/0000-0002-4643-7289>
  a owl:NamedIndividual ;
  a schema:Person ;
  schema:affiliation [
      schema:identifier "http://catalogue.linked.data.gov.au/org/ga"^^xsd:anyURI ;
      schema:name "Geoscience Australia" ;
    ] ;
  schema:email <mailto:irina.bastrakova@ga.gov.au> ;
  schema:identifier "https://orcid.org/0000-0002-4643-7289"^^xsd:anyURI ;
  schema:name "Irina Bastrakova"@en ;
.
<https://orcid.org/0000-0002-8742-7730>
  a owl:NamedIndividual ;
  a schema:Person ;
  schema:affiliation [
      schema:name "Surround Australia" ;
      schema:uri <https://surroundaustralia.com/> ;
    ] ;
  schema:email <mailto:nicholas.car@surroundaustralia.com> ;
  schema:identifier "https://orcid.org/0000-0002-8742-7730"^^xsd:anyURI ;
  schema:name "Nicholas Car"@en ;
.
<https://orcid.org/0000-0003-3425-0780>
  a owl:NamedIndividual ;
  a schema:Person ;
  schema:affiliation [
      schema:identifier "http://catalogue.linked.data.gov.au/org/anu"^^xsd:anyURI ;
      schema:name "Australian National University" ;
    ] ;
  schema:email <mailto:armin.haller@anu.edu.au> ;
  schema:identifier "https://orcid.org/0000-0003-3425-0780"^^xsd:anyURI ;
  schema:name "Armin Haller"@en ;
.
[
  dcterms:format <https://w3id.org/mediatype/text/html> ;
  prof:hasArtifact <http://linked.data.gov.au/def/placenames> ;
  prof:hasRole <http://www.w3.org/ns/dx/prof/role/specification> ;
].
[
  dcterms:format <https://w3id.org/mediatype/text/turtle> ;
  prof:hasArtifact <http://linked.data.gov.au/def/placenames.ttl> ;
  prof:hasRole <http://www.w3.org/ns/dx/prof/role/schema> ;
].
